% @author Shuning Zhang
% @date 2019-02-15
\documentclass[a4paper, 11pt]{ctexart}
\usepackage{amsfonts, amsmath, amssymb}
\usepackage{color}
\usepackage{enumerate}
\usepackage[bottom=2cm, left=2.5cm, right=2.5cm, top=2cm]{geometry}
\usepackage{multicol}
\begin{document}
\begin{enumerate}
    \item % 1
        $\overrightarrow{AB} = \dfrac12(\boldsymbol{a} - \boldsymbol{b})$,
        $\overrightarrow{BC} = \dfrac12(\boldsymbol{a} + \boldsymbol{b})$,
        $\overrightarrow{CD} = \dfrac12(\boldsymbol{b} - \boldsymbol{a})$,
        $\overrightarrow{DA} = -\dfrac12(\boldsymbol{a} + \boldsymbol{b})$.
    \item % 2
    
    \item % 3
        {\heiti 证明}\quad \begin{align*}
            \overrightarrow{AM} = \frac12\overrightarrow{AB}
            &\Leftrightarrow
            \overrightarrow{OM} - \overrightarrow{OA} = \frac12(\overrightarrow{OB} - \overrightarrow{OA}) \\
            &\Leftrightarrow
            \overrightarrow{OM} = \frac12(\overrightarrow{OA} + \overrightarrow{OB}).
        \end{align*}
    \item % 4
        {\heiti 证明}\quad \begin{align*}
            \overrightarrow{AM} = \frac12\overrightarrow{AC}
            &\Leftrightarrow
            \overrightarrow{OM} - \overrightarrow{OA} = \frac12(\overrightarrow{OC} - \overrightarrow{OA}) \\
            &\Leftrightarrow
            \overrightarrow{OM} = \frac12(\overrightarrow{OA} + \overrightarrow{OC}), \\
            \overrightarrow{BM} = \frac12\overrightarrow{BD}
            &\Leftrightarrow
            \overrightarrow{OM} - \overrightarrow{OB} = \frac12(\overrightarrow{OD} - \overrightarrow{OB}) \\
            &\Leftrightarrow
            \overrightarrow{OM} = \frac12(\overrightarrow{OB} + \overrightarrow{OD}).
        \end{align*}
        因此 $\overrightarrow{OM} = \dfrac14(\overrightarrow{OA} + \overrightarrow{OB} + \overrightarrow{OC} + \overrightarrow{OD})$.
    \item % 5
    \item % 6
    \item % 7
\end{enumerate}
\end{document}
